SeqPL/Kripke/Basic.lean
@@ -1,9 +1,9 @@
 module
 
-public import SeqPL.Formula
+public import SeqPL.Formula.Basic
 public import SeqPL.Vorspiel.CWF
 public import Mathlib.Data.PNat.Defs
-import Mathlib.Data.PNat.Basic
+public import Mathlib.Data.PNat.Basic
 
 @[expose]
 public section
